Fp/Tactics.lean
@@ -1,9 +1,8 @@
 import Lean
-
-register_simp_attr bv_float_normalize
+import Fp.Tactics.Attributes
+import Fp.Tactics.Simps
 
 syntax (name := bvFloat) "bv_float_normalize" : tactic
 
 macro_rules |
-  `(tactic| bv_float_normalize) => `(tactic| simp [bv_float_normalize,
-    -BitVec.shiftLeft_eq', -BitVec.ushiftRight_eq'] at *)
+  `(tactic| bv_float_normalize) => `(tactic| simp only [bv_float_normalize] at *)
