Fp/Tactics/Simps.lean
@@ -1,0 +1,9 @@
+import Fp.Tactics.Attributes
+
+attribute [bv_float_normalize] BitVec.setWidth'_eq
+attribute [bv_float_normalize] Eq.mp
+attribute [bv_float_normalize] ne_eq
+attribute [bv_float_normalize] beq_iff_eq
+attribute [bv_float_normalize] bne_iff_ne
+attribute [bv_float_normalize] Bool.or_eq_true
+attribute [bv_float_normalize] Bool.and_eq_true
